qed genie wp_checkDig. key idea: can't have wish include server pk good, since can't prove err = false -> pk good. instead, wish needs to be stuff implied from server pk good, like dig matches seenDigs

src/program_proof/pav/evidence.v
@@ -11,12 +11,12 @@ Record t :=
   }.
 Section defs.
 Context `{!heapGS Σ, !pavG Σ}.
-Definition own ptr obj : iProp Σ :=
+Definition own ptr obj d : iProp Σ :=
   ∃ ptr_sigDig0 ptr_sigDig1,
-  "#Hown_sigDig0" ∷ SigDig.own ptr_sigDig0 obj.(sigDig0) ∗
-  "Hptr_sigDig0" ∷ ptr ↦[Evid :: "sigDig0"] #ptr_sigDig0 ∗
-  "#Hown_sigDig1" ∷ SigDig.own ptr_sigDig1 obj.(sigDig1) ∗
-  "Hptr_sigDig1" ∷ ptr ↦[Evid :: "sigDig1"] #ptr_sigDig1.
+  "Hown_sigDig0" ∷ SigDig.own ptr_sigDig0 obj.(sigDig0) d ∗
+  "Hptr_sigDig0" ∷ ptr ↦[Evid :: "sigDig0"]{d} #ptr_sigDig0 ∗
+  "Hown_sigDig1" ∷ SigDig.own ptr_sigDig1 obj.(sigDig1) d ∗
+  "Hptr_sigDig1" ∷ ptr ↦[Evid :: "sigDig1"]{d} #ptr_sigDig1.
 End defs.
 End Evid.
 
@@ -24,7 +24,8 @@ Section defs.
 Context `{!heapGS Σ, !pavG Σ}.
 
 Definition is_SigDig obj pk : iProp Σ :=
-  is_sig pk (PreSigDig.encodesF (PreSigDig.mk obj.(SigDig.Epoch) obj.(SigDig.Dig))) obj.(SigDig.Sig).
+  is_sig pk (PreSigDig.encodesF
+    (PreSigDig.mk obj.(SigDig.Epoch) obj.(SigDig.Dig))) obj.(SigDig.Sig).
 
 Definition is_Evid obj pk : iProp Σ :=
   "#His_sigDig0" ∷ is_SigDig obj.(Evid.sigDig0) pk ∗
@@ -38,15 +39,16 @@ End defs.
 Section wps.
 Context `{!heapGS Σ, !pavG Σ}.
 
-Lemma wp_CheckSigDig ptr obj sl_pk pk :
+Lemma wp_CheckSigDig ptr obj sl_pk pk d0 :
   {{{
-    "#Hown_SigDig" ∷ SigDig.own ptr obj ∗
+    "Hown_SigDig" ∷ SigDig.own ptr obj d0 ∗
     "#Hsl_pk" ∷ own_slice_small sl_pk byteT DfracDiscarded pk
   }}}
   CheckSigDig #ptr (slice_val sl_pk)
   {{{
     (err : bool), RET #err;
-    "Hgenie" ∷ (is_SigDig obj pk ∗-∗ ⌜ err = false ⌝)
+    "Hgenie" ∷ (⌜ err = false ⌝ ∗-∗ is_SigDig obj pk) ∗
+    "Hown_SigDig" ∷ SigDig.own ptr obj d0
   }}}.
 Proof. Admitted.
 
