src/program_proof/pav/rpc.v
@@ -1,13 +1,13 @@
 From Perennial.program_proof Require Import grove_prelude.
 From Goose.github_com.mit_pdos.pav Require Import kt.
 
-From Perennial.program_proof.pav Require Import auditor advrpc core serde server.
+From Perennial.program_proof.pav Require Import auditor advrpc core cryptoffi serde server.
 
 Section specs.
 Context `{!heapGS Σ, !pavG Σ}.
 Lemma wp_NewRpcServer ptr_serv serv :
   {{{
-    "Hown_serv" ∷ server.Server.own ptr_serv serv
+    "Hserv" ∷ is_Server ptr_serv serv
   }}}
   NewRpcServer #ptr_serv
   {{{
@@ -18,7 +18,7 @@ Proof. Admitted.
 
 Lemma wp_NewRpcAuditor ptr_adtr :
   {{{
-    "Hown_adtr" ∷ Auditor.valid ptr_adtr
+    "Hadtr" ∷ Auditor.valid ptr_adtr
   }}}
   NewRpcAuditor #ptr_adtr
   {{{
@@ -39,9 +39,42 @@ Lemma wp_CallServPut ptr_cli cli (uid : w64) sl_pk d0 (pk : list w8) :
     "Hown_cli" ∷ advrpc.Client.own ptr_cli cli ∗
     "Hsl_pk" ∷ own_slice_small sl_pk byteT d0 pk ∗
     "Herr" ∷ (if err then True else
-      "#Hown_dig" ∷ SigDig.own ptr_dig dig ∗
-      "Hown_memb" ∷ Memb.own ptr_memb memb ∗
-      "Hown_nonmemb" ∷ NonMemb.own ptr_nonmemb nonmemb)
+      "Hown_dig" ∷ SigDig.own ptr_dig dig (DfracOwn 1) ∗
+      "Hown_memb" ∷ Memb.own ptr_memb memb (DfracOwn 1) ∗
+      "Hown_nonmemb" ∷ NonMemb.own ptr_nonmemb nonmemb (DfracOwn 1))
+  }}}.
+Proof. Admitted.
+
+(* TODO: properly bind serv record to rpc cli. *)
+Lemma wp_CallServPut_good ptr_cli cli serv uid nVers sl_pk d0 (pk : list w8) cli_ep :
+  {{{
+    "Hown_cli" ∷ advrpc.Client.own ptr_cli cli ∗
+    "Hvers" ∷ uid ↪[serv.(Server.γvers)] nVers ∗
+    "Hsl_pk" ∷ own_slice_small sl_pk byteT d0 pk ∗
+    "#Hlb_ep" ∷ mono_nat_lb_own serv.(Server.γepoch) cli_ep
+  }}}
+  CallServPut #ptr_cli #uid (slice_val sl_pk)
+  {{{
+    ptr_sigdig sigdig ptr_lat lat ptr_bound bound err,
+    RET (#ptr_sigdig, #ptr_lat, #ptr_bound, #err);
+    "Hown_cli" ∷ advrpc.Client.own ptr_cli cli ∗
+    "Hsl_pk" ∷ own_slice_small sl_pk byteT d0 pk ∗
+
+    "Hvers" ∷ uid ↪[serv.(Server.γvers)] (word.add nVers (W64 1)) ∗
+    "%Heq_ep" ∷ ⌜ sigdig.(SigDig.Epoch) = lat.(Memb.EpochAdded) ⌝ ∗
+    "%Heq_pk" ∷ ⌜ pk = lat.(Memb.PkOpen).(CommitOpen.Val) ⌝ ∗
+    "#Hlb_ep" ∷ mono_nat_lb_own serv.(Server.γepoch) (uint.nat sigdig.(SigDig.Epoch)) ∗
+    "%Hlt_ep" ∷ ⌜ Z.of_nat cli_ep < uint.Z sigdig.(SigDig.Epoch) ⌝ ∗
+    "#Hsigdig" ∷ SigDig.own ptr_sigdig sigdig DfracDiscarded ∗
+    "#Hsig" ∷ is_sig serv.(Server.sig_pk)
+      (PreSigDig.encodesF $ PreSigDig.mk sigdig.(SigDig.Epoch) sigdig.(SigDig.Dig))
+      sigdig.(SigDig.Sig) ∗
+    "Hlat" ∷ Memb.own ptr_lat lat (DfracOwn 1) ∗
+    "#Hwish_lat" ∷ wish_memb serv.(Server.vrf_pk) uid nVers sigdig lat ∗
+    "Hbound" ∷ NonMemb.own ptr_bound bound (DfracOwn 1) ∗
+    "#Hwish_bound" ∷ wish_nonmemb serv.(Server.vrf_pk)
+      uid (word.add nVers (W64 1)) sigdig bound ∗
+    "->" ∷ ⌜ err = false ⌝
   }}}.
 Proof. Admitted.
 
@@ -55,12 +88,11 @@ Lemma wp_CallServGet ptr_cli cli (uid : w64) :
     RET (#ptr_dig, slice_val sl_hist, #is_reg, #ptr_memb, #ptr_nonmemb, #err);
     "Hown_cli" ∷ advrpc.Client.own ptr_cli cli ∗
     "Herr" ∷ (if err then True else
-      "#Hown_dig" ∷ SigDig.own ptr_dig dig ∗
+      "#Hown_dig" ∷ SigDig.own ptr_dig dig (DfracOwn 1) ∗
       "Hsl_hist" ∷ own_slice_small sl_hist ptrT (DfracOwn 1) hist_ref ∗
-      "Hown_hist" ∷ ([∗ list] l;v ∈ hist_ref;hist, MembHide.own l v) ∗
-      "Hown_memb" ∷ Memb.own ptr_memb memb ∗
-      "%Hpk_dfrac" ∷ ⌜ memb.(Memb.PkOpen).(CommitOpen.d) = DfracOwn 1 ⌝ ∗
-      "Hown_nonmemb" ∷ NonMemb.own ptr_nonmemb nonmemb)
+      "Hown_hist" ∷ ([∗ list] l;v ∈ hist_ref;hist, MembHide.own l v (DfracOwn 1)) ∗
+      "Hown_memb" ∷ Memb.own ptr_memb memb (DfracOwn 1) ∗
+      "Hown_nonmemb" ∷ NonMemb.own ptr_nonmemb nonmemb (DfracOwn 1))
   }}}.
 Proof. Admitted.
 
@@ -73,8 +105,8 @@ Lemma wp_CallServSelfMon ptr_cli cli (uid : w64) :
     (err : bool) ptr_dig dig ptr_nonmemb nonmemb, RET (#ptr_dig, #ptr_nonmemb, #err);
     "Hown_cli" ∷ advrpc.Client.own ptr_cli cli ∗
     "Herr" ∷ (if err then True else
-      "#Hown_dig" ∷ SigDig.own ptr_dig dig ∗
-      "Hown_nonmemb" ∷ NonMemb.own ptr_nonmemb nonmemb)
+      "#Hown_dig" ∷ SigDig.own ptr_dig dig (DfracOwn 1) ∗
+      "Hown_nonmemb" ∷ NonMemb.own ptr_nonmemb nonmemb (DfracOwn 1))
   }}}.
 Proof. Admitted.
 
@@ -87,21 +119,21 @@ Lemma wp_CallServAudit ptr_cli cli (ep : w64) :
     (err : bool) ptr_upd upd, RET (#ptr_upd, #err);
     "Hown_cli" ∷ advrpc.Client.own ptr_cli cli ∗
     if negb err then
-      "Hown_upd" ∷ UpdateProof.own ptr_upd upd
+      "Hown_upd" ∷ UpdateProof.own ptr_upd upd (DfracOwn 1)
     else True
   }}}.
 Proof. Admitted.
 
-Lemma wp_CallAdtrUpdate ptr_cli cli ptr_upd upd :
+Lemma wp_CallAdtrUpdate ptr_cli cli ptr_upd upd d0 :
   {{{
     "Hown_cli" ∷ advrpc.Client.own ptr_cli cli ∗
-    "Hown_upd" ∷ UpdateProof.own ptr_upd upd
+    "Hown_upd" ∷ UpdateProof.own ptr_upd upd d0
   }}}
   CallAdtrUpdate #ptr_cli #ptr_upd
   {{{
     (err : bool), RET #err;
     "Hown_cli" ∷ advrpc.Client.own ptr_cli cli ∗
-    "Hown_upd" ∷ UpdateProof.own ptr_upd upd
+    "Hown_upd" ∷ UpdateProof.own ptr_upd upd d0
   }}}.
 Proof. Admitted.
 
@@ -114,7 +146,7 @@ Lemma wp_CallAdtrGet ptr_cli cli (ep : w64) :
     (err : bool) ptr_adtrInfo adtrInfo, RET (#ptr_adtrInfo, #err);
     "Hown_cli" ∷ advrpc.Client.own ptr_cli cli ∗
     if negb err then
-      "Hown_info" ∷ AdtrEpochInfo.own ptr_adtrInfo adtrInfo
+      "Hown_info" ∷ AdtrEpochInfo.own ptr_adtrInfo adtrInfo (DfracOwn 1)
     else True
   }}}.
 Proof. Admitted.
